compiler/backend/languages/pure_cexpScript.sml
@@ -75,6 +75,8 @@ Datatype:
                                         (* case w/non-empty pattern-exp list *)
 End
 
+val cexp_size_eq = fetch "-" "cexp_size_eq";
+
 Theorem cexp_size_lemma:
   (∀xs a. MEM a xs ⇒ cexp_size f a < cexp10_size f xs) ∧
   (∀xs p e. MEM (p,e) xs ⇒ cexp_size f e < cexp6_size f xs) ∧
@@ -284,6 +286,35 @@ Definition NestedCase_free_def[simp]:
 Termination
   WF_REL_TAC ‘measure $ cexp_size (K 0)’ >>
   simp[fetch "-" "cexp_size_eq", MEM_MAP, PULL_EXISTS, FORALL_PROD] >> rw[] >>
+  rename [‘MEM _ list’] >> Induct_on ‘list’ >>
+  simp[FORALL_PROD, listTheory.list_size_def, basicSizeTheory.pair_size_def] >>
+  rw[] >> gs[]
+End
+
+Definition every_cexp_def[simp]:
+  every_cexp (p:'a cexp -> bool) (Var a v) = p (Var a v) ∧
+  every_cexp p (Prim a x es) =
+    (p (Prim a x es) ∧ EVERY (every_cexp p) es) ∧
+  every_cexp p (App a e es) =
+    (p (App a e es) ∧ every_cexp p e ∧ EVERY (every_cexp p) es) ∧
+  every_cexp p (Lam a vs e) =
+    (p (Lam a vs e) ∧ every_cexp p e) ∧
+  every_cexp p (Let a v e1 e2) =
+    (p (Let a v e1 e2) ∧ every_cexp p e1 ∧ every_cexp p e2) ∧
+  every_cexp p (Letrec a fns e) =
+    (p (Letrec a fns e) ∧
+     every_cexp p e ∧ EVERY (every_cexp p) $ MAP SND fns) ∧
+  every_cexp p (Case a e v css eopt) =
+    (p (Case a e v css eopt) ∧
+     every_cexp p e ∧ EVERY (every_cexp p) $ MAP (SND o SND) css ∧
+     OPTION_ALL (every_cexp p o SND) eopt) ∧
+  every_cexp p (NestedCase a e1 v pat e2 rows) =
+    (p (NestedCase a e1 v pat e2 rows) ∧
+     every_cexp p e1 ∧ every_cexp p e2 ∧
+     EVERY (every_cexp p) $ MAP SND rows)
+Termination
+  WF_REL_TAC ‘measure $ cexp_size (K 0) o SND’ >>
+  simp[cexp_size_eq, MEM_MAP, PULL_EXISTS, FORALL_PROD] >> rw[] >>
   rename [‘MEM _ list’] >> Induct_on ‘list’ >>
   simp[FORALL_PROD, listTheory.list_size_def, basicSizeTheory.pair_size_def] >>
   rw[] >> gs[]
